examples/Sek/PSek.ml
@@ -6,15 +6,10 @@ type 'a psek = {
   mid : 'a pchunk psek option
 }
 
-let psek_default =
-  pchunk_default sides.(0)
+let psek_default c =
+  pchunk_default c.sides.(0)
 
 let psek_create d = {
   sides = [| pchunk_create d; pchunk_create d |];
   mid = None
 }
-
-let psek_is_empty =
-  match mid with
-  | None -> pchunk_is_empty sides.(0) && pchunk_is_empty sides.(1)
-  | Some _ -> false
