examples/Sek/Capacity_proof.v
@@ -1,0 +1,73 @@
+Set Implicit Arguments.
+From CFML Require Import LibSepGroup WPLibCredits Stdlib.
+Open Scope cf_scope.
+Open Scope record_scope.
+
+Require Import Capacity_ml.
+
+
+(* ******************************************************* *)
+(** ** Definitions *)
+
+Notation "'K'" := capacity.
+
+Definition Wrap_up i := If i >= K then i - K else i.
+Definition Wrap_down i := If i < 0 then i + K else i.
+
+
+(* ******************************************************* *)
+(** ** Lemma *)
+
+Lemma capacity_spec :
+  capacity > 0.
+Proof. rewrite capacity_cf__; math. Qed.
+
+(* ******************************************************* *)
+(** ** Hints *)
+
+Hint Extern 1 (@le _ _ _ capacity) => hint capacity_spec; math.
+Hint Extern 1 (@lt _ _ _ capacity) => hint capacity_spec; math.
+Hint Extern 1 (@ge _ _ capacity _) => hint capacity_spec; math.
+Hint Extern 1 (@gt _ _ capacity _) => hint capacity_spec; math.
+
+
+(* ******************************************************* *)
+(** ** Tactics *)
+
+Tactic Notation "unwrap_up" :=
+	unfold Wrap_up; repeat case_if*.
+Tactic Notation "unwrap_up" "in" hyp(H) :=
+	unfold Wrap_up in H; repeat case_if* in H.
+
+Tactic Notation "unwrap_down" :=
+	unfold Wrap_down; repeat case_if*.
+Tactic Notation "unwrap_down" "in" hyp(H) :=
+	unfold Wrap_down in H; repeat case_if* in H.
+
+
+(* ******************************************************* *)
+(** ** Specifications *)
+
+Lemma wrap_up_spec : forall (n: int),
+	SPEC (wrap_up n)
+		PRE (\$1)
+		POST (fun n' => \[n' = Wrap_up n]).
+Proof.
+	xcf. unfold Wrap_up.
+	xpay.
+	xif; intros C; case_if; xval*; xsimpl*.
+Qed.
+
+Hint Extern 1 (RegisterSpec wrap_up) => Provide wrap_up_spec.
+
+Lemma wrap_down_spec : forall (n: int),
+	SPEC (wrap_down n)
+		PRE (\$1)
+		POST (fun n' => \[n' = Wrap_down n]).
+Proof.
+	xcf. unfold Wrap_down.
+	xpay.
+	xif; intros C; case_if; xval*; xsimpl*.
+Qed.
+
+Hint Extern 1 (RegisterSpec wrap_down) => Provide wrap_down_spec.
